add systemf/autosubst2 type safety

systemf/lngen/def_extra.v
@@ -7,6 +7,15 @@ Inductive ctx_entry :=
 
 Definition ctx := list (atom * ctx_entry).
 
+Ltac gather_atoms ::=
+  let A := gather_atoms_with (fun x : vars => x) in
+  let B := gather_atoms_with (fun x : var => {{ x }}) in
+  let C1 := gather_atoms_with (fun x : exp => var_in_exp x) in
+  let C2 := gather_atoms_with (fun x : exp => tvar_in_exp x) in
+  let D := gather_atoms_with (fun x : typ => tvar_in_typ x) in
+  let DE:= gather_atoms_with (fun x : ctx => dom x) in
+  constr:(A \u B \u C1 \u C2 \u D \u D).
+
 Reserved Notation "Γ ⊢ t : A" 
   (at level 50, t at next level, no associativity).
 Inductive typing : ctx -> exp -> typ -> Prop :=
@@ -29,3 +38,29 @@ Inductive typing : ctx -> exp -> typ -> Prop :=
   Γ ⊢ t : (typ_all A) ->
   Γ ⊢ exp_tapp t B : (open_typ_wrt_typ A B)
 where "Γ ⊢ t : A" := (typing Γ t A).
+
+Definition is_value (t : exp) : Prop :=
+  match t with
+  | exp_abs _ _ => True
+  | exp_tabs _ => True
+  | _ => False
+  end.
+
+Reserved Notation "t ⤳ t'" (at level 80).
+Inductive step : exp -> exp -> Prop :=
+| step_appl t t' s : 
+  t ⤳ t' -> 
+  exp_app t s ⤳ exp_app t' s
+| step_appr t s s' : 
+  is_value t ->
+  s ⤳ s' -> 
+  exp_app t s ⤳ exp_app t s'
+| step_beta t s A : 
+  is_value s ->
+  exp_app (exp_abs A t) s ⤳ open_exp_wrt_exp t s
+| step_tapp t t' A : 
+  t ⤳ t' ->
+  exp_tapp t A ⤳ exp_tapp t' A
+| step_inst t A: 
+  exp_tapp (exp_tabs t) A ⤳ open_exp_wrt_typ t A
+where "t ⤳ t'" := (step t t').
